\section{Семинар}

\subsection{Задача \textnumero2.12}
\paragraph{Условие}
Решить задачу Коши: $y' = \sqrt{x}, y(0) = -1$
\paragraph{Решение}
\begin{gather*}
	y' = \sqrt{x} \\
	y = \int \sqrt{x}dx
	y = \int x^{1/2}dx
	y = \frac{x^{3/2}}{3/2} + C
	y = \frac{2x^{3/2}}{3} + C
\end{gather*}
Если $y(0) = -1$:
\begin{gather*}
	y(0) = \frac{2 \cdot 0^{3/2}}{3} + C = -1
	C = -1
\end{gather*}
Таким образом, \textit{частичное решение}:
\[y = \frac{2x^{3/2}}{3} - 1\]

\subsection{Задача \textnumero2.21}
\paragraph{Условие}
Решить дифференциальное уравнение: $2y'\sqrt{x} = y, y(4) = 1$
\paragraph{Решение}
\begin{gather*}
	2y'\sqrt{x} = y \\
	2 \frac{dy}{dx} \sqrt{x} = y \\
	\frac{2\sqrt{x}}{dx} = \frac{y}{dy} \\
	\frac{dx}{2\sqrt{x}} = \frac{dy}{y} \\
\end{gather*}
\begin{gather*}
	\frac{1}{2} \int \frac{dx}{\sqrt{x}} = \int \frac{dy}{y} \\
	\frac{1}{2} \frac{x^{1/2}}{1/2} + C = \ln{y} \\
	\frac{1}{2} 2x^{1/2} + C = \ln{y} \\
	\sqrt{x} + C = \ln{y} \\
	y = e^{\sqrt{x} + C} \\
	y = e^{\sqrt{x}} \cdot e^C \\
	y = Ce^{\sqrt{x}} \\
\end{gather*}
Если $y(4) = 1$:
\begin{gather*}
	y(4) = Ce^{\sqrt{4}} = 1 \\
	Ce^2 = 1 \\
	C = \frac{1}{e^2}
\end{gather*}
Таким образом, \textit{частичное решение}:
\[y = e^{\sqrt{x} - 2}\]
