\section{Лекция}

\subsection{Задание \textnumero1}
\paragraph{Условие}
Решит лин. однородн. диф. ур. 1-го порядка: $y' - 2y = 2e^{2x}$ методом \textit{вариации постоянных}
\paragraph{Решение}
\begin{equation} \label{eq:initial}
	y' - 2y = 2e^{2x} \\
\end{equation}
Рассмотрим \textit{соответсвующее} лин. однородн. диф. ур. $y' - 2y = 0$:
\begin{gather*}
	y' = 2y \\
	\frac{dy}{dx} = 2y \\
	\frac{dy}{y} = 2dx \\
	\int \frac{dy}{y} = \int 2dx \\
	\int \frac{dy}{y} = 2\int dx \\
	\ln{y} = 2x + C_1 \\
	\lvert y \rvert = e^{2x+C_1} \\
	y = \pm e^{2x} \cdot e^C_1 \\
	y = C_1e^{2x}, C_1 \in \mathbb{R}
\end{gather*}
\begin{equation}
	y = C_1e^{2x}, C_1 \in \mathbb{R}
	\label{eq:partial}
\end{equation}

Решим \ref{eq:initial}, подставим $y$:
\begin{gather*}
	(C_1(x)e^{2x})' - 2C_1(x)e^{2x} = 2e^{2x} \\
	C_1'(x)e^{2x} + 2C_1(x)e^{2x} - 2C_1(x)e^{2x} = 2e^{2x} \\
	C_1'(x)e^{2x} = 2e^{2x} \\
	C_1'(x) = 2 \\
	C_1(x) = \int2dx \\
	C_1(x) = 2x  + C_2 \\
\end{gather*}

Подставим $C_1$ в \ref{eq:partial}
\[y = (2x  + C_2) \cdot e^{2x} \]
\begin{equation}
	y = 2xe^{2x}  + C_2e^{2x} \\
	\label{eq:solution}
\end{equation}

Проверим путем подстановки:
\begin{gather*}
	(2xe^{2x}  + C_2e^{2x})' - 2(2xe^{2x}  + C_2e^{2x}) = 2e^{2x} \\
	2C_2e^{2x} + 2e^{2x} + 4xe^{2x} - 2C_2e^{2x} - 4xe^{2x} = 2e^{2x} \\
	2e^{2x} = 2e^{2x} \\
\end{gather*}
Следовательно, $y = 2xe^{2x}  + C_2e^{2x}$ - общее решение \ref{eq:initial}

\subsection{Задание \textnumero2}
\paragraph{Условие}
\[y' - 2y = 2e^{2x}\]
\paragraph{Решение}
\begin{gather*}
\end{gather*}
