%hello
\section{Семинар 2. Раздностгые уравнения}

\subsection{Задача 9.1}
\[y_{k_2} + y_{k+1} - 2y_k = 0\]
\subsection{Решение}
\begin{gather*}
	y = \lambda^k \\
	\lambda^{k+2} + \lambda^{k+1} - 2\lambda^k = 0 \\
	\lambda^k(\lambda^2 + labda - 2) = 0, \lambda^k \neq 0 \\
	\lambda_1 = 1, \lambda_2 = -2 \\
	y_1 = q^k, y_2 = (-2)^k \textup{ --- реш. разност. уравн.} \\
	y_k = C_1 \cdot 1^k + C_2 \cdot (-2)^k \textup{ --- ответ}
\end{gather*}

\subsection{Задача 9.6}
\[y_{k+2} - 4y_{k+1} + 4y_k = 0\]
\subsection{Решение}
\begin{gather*}
	\lambda^2 - t\lambda + 4 = 0 \\
	\lambda_{1,2} = 2 \\
	\begin{cases}
		y_1 = 2^k \\
		y_2 = k \cdot 2^k
	\end{cases} \\
	y_k = C_1 \cdot 2^k + C_2 \cdot 2^kk = 2^k(C_1+kC_2) \textup{ --- ответ}
\end{gather*}

\subsection{Задача 9.11}
\[y_{k+2} - 2y_{k+1} + 4y_k = 0\]
\subsection{Решение}
\begin{gather*}
	y = \lambda^k \\
	\lambda^2 - 2\lambda + 4 = 0 \\
	\frac{D}{4} = 1 - 4 = -3 \\
	\lambda_{1,2} = 1 \pm \sqrt{-3} \\
	\lambda_{1,2} = 1 \pm i\sqrt{3} \\
	y_{k} = \rho^k(C_1\cos{k\phi} + C_2\sin{k\phi}), \\
	\rho = \sqrt{1^2 + \sqrt{3}^2}, \phi = arctg{\frac{b}{a}} = \frac{\pi}{3} \\
	y_{k} = 2^k\left(C_1\cos{k\frac{\pi}{3}} + C_2\sin{k\frac{\pi}{3}}\right) \\
\end{gather*}
